SSA/Experimental/Bits/Fast/Tests.lean
@@ -64,9 +64,17 @@ example (w : Nat) (a b : BitVec w) : a + b = b + a := by
 example (w : Nat) (a b : BitVec w) : (a + b = b + a)  := by
   bv_automata_gen (config := {backend := .circuit_cadical_verified} )
 
+set_option trace.Bits.FastVerif true in
+example (w : Nat) (a : BitVec w) : (a ≠ a) := by
+  -- not true at 0.
+  fail_if_success bv_automata_gen (config := {backend := .circuit_cadical_verified (maxIter := 7) (version := .V2) } )
+  sorry
+
+set_option trace.Bits.FastVerif true in
 example (w : Nat) (a : BitVec w) : (a = a + 0#w) ∨ (a = a - a)  := by
-  fail_if_success bv_automata_gen (config := {backend := .circuit_cadical_verified 20 } )
-  bv_automata_gen (config := {backend := .circuit_cadical_unverified 20 } )
+  -- fail_if_success bv_automata_gen (config := {backend := .circuit_cadical_verified 20 } )
+  bv_automata_gen (config := {backend := .circuit_cadical_verified (maxIter := 7) (version := .V2) } )
+  -- bv_automata_gen (config := {backend := .circuit_cadical_unverified 20 } )
 
 example (w : Nat) (a : BitVec w) :  (a = a + 0#w)  := by
   bv_automata_gen (config := {backend := .circuit_cadical_verified 20 } )
@@ -106,7 +114,7 @@ example (w : Nat) (a : BitVec w) : (a = 0#w) ∨ (a = a + 0#w)  := by
 set_option trace.Bits.FastVerif true in
 example (w : Nat) (a : BitVec w) : a = 1#w   := by
   fail_if_success bv_automata_gen (config := {backend := .circuit_cadical_verified 20 (version := .V2) } )
-
+  sorry
 
 example (w : Nat) (a b : BitVec w) : (a = 0#w) ∨ (a + b = b + a) := by
   -- bv_automata_gen (config := {backend := .circuit_cadical_verified} )
@@ -298,6 +306,9 @@ def test11 (x y : BitVec w) : (x + y) = ((x |||  y) +  (x &&&  y)) := by
 def test15 (x y : BitVec w) : (x - y) = (( x &&& (~~~ y)) - ((~~~ x) &&&  y)) := by
   bv_automata_gen (config := {backend := .circuit_cadical_verified} )
 
+def test15' (x y : BitVec w) : (x - y) = (( x &&& (~~~ y)) - ((~~~ x) &&&  y)) := by
+  bv_automata_gen (config := {backend := .circuit_cadical_verified (version := .V2) } )
+
 def test17 (x y : BitVec w) : (x ^^^ y) = ((x ||| y) - (x &&& y)) := by
   bv_automata_gen (config := {backend := .circuit_cadical_verified} )
 
@@ -400,6 +411,7 @@ theorem mul_eleven (x : BitVec w) : 11 * x =
   (x + x + x + x + x +
    x + x + x + x + x +
    x) := by
+  -- bv_automata_gen (config := {backend := .circuit_cadical_verified 6 .V2 } )
   bv_automata_gen (config := {backend := .circuit_cadical_verified 6 } )
 
 theorem mul_eleven' (x : BitVec w) : 11 * x =
@@ -460,16 +472,17 @@ theorem e_1 (x y : BitVec w) :
      - 1 *  ~~~(x ^^^ y) - 2 * y + 1 *  ~~~x =  - 1 *  ~~~(x |||  ~~~y) - 3 * (x &&& y) := by
   bv_automata_gen (config := {backend := .circuit_cadical_verified 5 } )
 
+set_option trace.Bits.FastVerif true in
 theorem e_331 (x y : BitVec w):
      - 6 *  ~~~x + 2 * (x |||  ~~~y) - 3 * x + 2 * (x ||| y) - 10 *  ~~~(x ||| y) - 10 *  ~~~(x |||  ~~~y) - 4 * (x &&&  ~~~y) - 15 * (x &&& y) + 3 *  ~~~(x &&&  ~~~x) + 11 *  ~~~(x &&&  ~~~y) = 0#w := by
   -- bv_automata_gen (config := {genSizeThreshold := 2000, stateSpaceSizeThreshold := 100})
-  fail_if_success bv_automata_gen (config := {backend := .circuit_cadical_verified 5 } )
-  bv_automata_gen (config := {backend := .circuit_cadical_unverified 5 } )
+  bv_automata_gen (config := {backend := .circuit_cadical_verified 6 (version := .V2) } )
+  -- bv_automata_gen (config := {backend := .circuit_cadical_unverified 5 } )
 
 set_option maxHeartbeats 0 in
 theorem e_2500 (a b c d e f g h i j k l m n o p q r s t u v x y z : BitVec w):
     7 * ( ~~~f ||| (d ^^^ e)) - 6 * ( ~~~(d &&&  ~~~e) &&& (e ^^^ f)) - 11 * ( ~~~(d &&&  ~~~e) &&& (d ^^^ (e ^^^ f))) - 1 * (f ^^^  ~~~( ~~~d &&& (e ||| f))) + 3 * ((e &&&  ~~~f) |||  ~~~(d ||| ( ~~~e &&& f))) - 3 * (f |||  ~~~(d |||  ~~~e)) + 1 *  ~~~(e ^^^ f) + 1 *  ~~~(d &&& (e ||| f)) + 5 * ( ~~~(d |||  ~~~e) ||| (d ^^^ (e ^^^ f))) + 1 * (e ^^^  ~~~(d ||| (e &&& f))) + 1 *  ~~~(d ||| ( ~~~e &&& f)) - 1 * ( ~~~d ||| (e ^^^ f)) + 4 * (e ^^^  ~~~( ~~~d &&& (e ||| f))) + 3 * ((d &&&  ~~~e) |||  ~~~(e ^^^ f)) + 4 * (f ^^^ ( ~~~d ||| ( ~~~e ||| f))) + 4 * ((e &&&  ~~~f) ^^^ (d ||| (e ^^^ f))) + 7 * ((d &&&  ~~~e) ||| (e ^^^ f)) + 2 * ((d ||| e) &&& (e ^^^ f)) + 3 * (e ^^^  ~~~( ~~~d ||| (e ^^^ f))) - 6 * (e ^^^  ~~~(d &&& f)) - 1 * (e ^^^ ( ~~~d ||| (e ||| f))) + 5 * (f ^^^ (d &&& (e ||| f))) + 4 * ((d &&& f) ^^^ (e ||| f)) + 1 * (e &&& (d |||  ~~~f)) - 2 *  ~~~(d &&&  ~~~e) + 7 * (f ^^^  ~~~( ~~~d &&& ( ~~~e ||| f))) - 3 * ((d &&& e) |||  ~~~(e ^^^ f)) - 1 *  ~~~( ~~~d &&& ( ~~~e ||| f)) - 5 * (f ^^^ ( ~~~d ||| (e &&& f))) - 1 * (d ||| (e ||| f)) + 5 * (d &&&  ~~~f) + 7 * (f ||| (d &&& e)) - 1 * ( ~~~d &&& (e ||| f)) + 1 * ( ~~~(d ||| e) ||| (d ^^^ (e ^^^ f))) + 7 * (e ^^^  ~~~( ~~~d &&& (e ^^^ f))) + 1 * ((d |||  ~~~e) &&& (d ^^^ (e ^^^ f))) + 11 *  ~~~(d ||| (e ^^^ f)) + 4 * (e ^^^ (d &&& (e ^^^ f))) - 1 * ( ~~~d ||| ( ~~~e ||| f)) + 5 * ((d &&&  ~~~e) |||  ~~~(d ^^^ (e ^^^ f))) - 11 * (e ^^^ ( ~~~d ||| (e ^^^ f))) - 1 * (d &&& (e ||| f)) - 1 * (f ^^^  ~~~( ~~~d ||| ( ~~~e &&& f))) + 3 * (e ^^^ ( ~~~d &&& (e ||| f))) + 7 * (e ^^^ (d &&&  ~~~f)) + 1 *  ~~~( ~~~d &&& ( ~~~e &&& f)) - 1 * (e ^^^ (d ||| (e &&& f))) + 1 * (e ^^^ (d &&& ( ~~~e ||| f))) - 1 * (f ^^^ ( ~~~d &&& ( ~~~e ||| f))) - 1 * (d ||| ( ~~~e &&& f)) - 6 * (e ^^^  ~~~(d |||  ~~~f)) + 3 *  ~~~(d ||| f) + 4 * (e |||  ~~~(d ^^^ f)) - 2 *  ~~~(d &&& ( ~~~e ||| f)) - 6 * f - 1 * (e |||  ~~~(d |||  ~~~f)) + 5 * ((d ^^^ e) |||  ~~~(d ^^^ f)) - 2 * (f ^^^ ( ~~~d ||| (e ||| f))) + 5 * (f ^^^  ~~~(d |||  ~~~e)) - 11 * (e ||| (d &&&  ~~~f)) + 11 *  ~~~(d &&& (e &&& f)) - 3 * (e ^^^  ~~~( ~~~d &&& ( ~~~e ||| f))) - 5 * ((d &&& e) ||| (e ^^^ f)) + 1 * ((e &&&  ~~~f) ^^^ ( ~~~d ||| (e ^^^ f))) - 3 * (f ^^^  ~~~(d &&& ( ~~~e &&& f))) - 1 *  ~~~(d &&& ( ~~~e &&& f)) + 4 *  ~~~( ~~~d &&& (e &&& f)) - 6 * ((d ||| e) &&&  ~~~(e ^^^ f)) - 11 * ( ~~~e &&& (d ^^^ f)) - 7 * (f &&& (d |||  ~~~e)) + 5 * (d &&& ( ~~~e ||| f)) + 11 *  ~~~(e ||| f) - 7 * (f ^^^  ~~~(d &&& e)) + 1 * ((d ^^^ e) &&& (d ^^^ f)) - 39 *  ~~~(d ||| (e ||| f)) - 29 *  ~~~(d ||| ( ~~~e ||| f)) - 54 *  ~~~( ~~~d ||| (e ||| f)) - 32 *  ~~~( ~~~d ||| ( ~~~e ||| f)) + 19 * ( ~~~d &&& ( ~~~e &&& f)) - 60 * ( ~~~d &&& (e &&& f)) - 31 * (d &&& ( ~~~e &&& f)) + 33 * (d &&& (e &&& f)) =  - 1 * (e ^^^  ~~~( ~~~d ||| ( ~~~e &&& f))) + 3 *  ~~~(d ^^^ f) := by
-  bv_automata_gen (config := {backend := .circuit_cadical_verified 20 (version := .V2) } )
+  bv_automata_gen (config := {backend := .circuit_cadical_verified 3 (version := .V2) } )
 
 #exit
 
